lava/out/Benchmark/PLE/MonoidMaybe.v
@@ -1,60 +1,52 @@
 From coqDeps Require Export LiquidPreludeUtil.
 Open Scope Z_scope.
 Open Scope Int_scope.
-Inductive Maybe_u : Set := 
-	 | Just_u: Z -> Maybe_u
-	 | Nothing_u: Maybe_u
-	 | Nothing_u: Maybe_u. 
-Fixpoint Maybe_eq (x: Maybe_u) (y: Maybe_u): bool := 
-	match (x, y) with (Just_u x, Just_u x') => (true && (x ==? x')) | (Nothing_u, Nothing_u) => true | (Nothing_u, Nothing_u) => true | (_, _) => false end. 
-Definition Maybe_eq_refl: (forall (x: Maybe_u) , is_true (Maybe_eq x x)). 
+Inductive MaybeInt_u : Set := 
+	 | Just_u: Z -> MaybeInt_u
+	 | Nothing_u: MaybeInt_u. 
+Fixpoint MaybeInt_eq (x: MaybeInt_u) (y: MaybeInt_u): bool := 
+	match (x, y) with (Just_u x, Just_u x') => (true && (x ==? x')) | (Nothing_u, Nothing_u) => true | (_, _) => false end. 
+Definition MaybeInt_eq_refl: (forall (x: MaybeInt_u) , is_true (MaybeInt_eq x x)). 
 Proof. 
 	eq_refl. 
 Qed. 
-#[global] Hint Resolve Maybe_eq_refl : eq_hint_db.
-Definition Maybe_eqb_eq: (forall (s: Maybe_u) (t: Maybe_u) , (is_true (Maybe_eq s t)) -> (s = t)). 
+#[global] Hint Resolve MaybeInt_eq_refl : eq_hint_db.
+Definition MaybeInt_eqb_eq: (forall (s: MaybeInt_u) (t: MaybeInt_u) , (is_true (MaybeInt_eq s t)) -> (s = t)). 
 Proof. 
 	eqb_eq_lem. 
 Qed. 
-#[global] Hint Resolve Maybe_eqb_eq : eq_hint_db.
-#[global] Instance leibnitz_eq_Maybe : LeibnitzEqB := { 
-	equalB' := Maybe_eq;
-	refl' := Maybe_eq_refl;
-	eqb_eq' := Maybe_eqb_eq
+#[global] Hint Resolve MaybeInt_eqb_eq : eq_hint_db.
+#[global] Instance leibnitz_eq_MaybeInt : LeibnitzEqB := { 
+	equalB' := MaybeInt_eq;
+	refl' := MaybeInt_eq_refl;
+	eqb_eq' := MaybeInt_eqb_eq
 }.
-Fixpoint Maybe_wf (x: Maybe_u): Prop := 
-	match x with (Just_u VV) => True | Nothing_u => True | Nothing_u => True end. 
-Theorem Maybe_wf_ref [p: Maybe_u -> Prop] (tm: {v: Maybe_u | (Maybe_wf v) /\ (p v)}): Maybe_wf (⌊ tm -⌋). 
+Fixpoint MaybeInt_wf (x: MaybeInt_u): Prop := 
+	match x with (Just_u VV) => True | Nothing_u => True end. 
+Theorem MaybeInt_wf_ref [p: MaybeInt_u -> Prop] (tm: {v: MaybeInt_u | (MaybeInt_wf v) /\ (p v)}): MaybeInt_wf (⌊ tm -⌋). 
 Proof. 
 	destruct tm as [tm tm_p]. 
 	solver. 
 Qed. 
-Global Notation Maybe := {x: Maybe_u | (Maybe_wf x) /\ True}. 
-Definition Just_lem (VV: {VV: Z | True}): (Maybe_wf (Just_u (⌊ VV -⌋))) /\ True. 
+Global Notation MaybeInt := {x: MaybeInt_u | (MaybeInt_wf x) /\ True}. 
+Definition Just_lem (VV: {VV: Z | True}): (MaybeInt_wf (Just_u (⌊ VV -⌋))) /\ True. 
 Proof. 
 	repeat first [split; solver]. 
 Defined. 
-Definition Just (VV: {VV: Z | True}): Maybe := 
+Definition Just (VV: {VV: Z | True}): MaybeInt := 
 	exist _ (Just_u (⌊ VV -⌋)) (Just_lem VV). 
-Definition Nothing_lem: (Maybe_wf Nothing_u) /\ True. 
+Definition Nothing_lem: (MaybeInt_wf Nothing_u) /\ True. 
 Proof. 
 	repeat first [split; solver]. 
 Defined. 
-Definition Nothing: Maybe := 
+Definition Nothing: MaybeInt := 
 	exist _ Nothing_u Nothing_lem. 
-Definition Nothing_lem: (Maybe_wf Nothing_u) /\ True. 
-Proof. 
-	repeat first [split; solver]. 
-Defined. 
-Definition Nothing: Maybe := 
-	exist _ Nothing_u Nothing_lem. 
-#[global] Hint Resolve Maybe_wf_ref : wf_constr_db.
-#[global] Hint Unfold Maybe_wf : wf_constr_db.
-#[global] Hint Resolve Maybe_eq : ref_constr_db.
+#[global] Hint Resolve MaybeInt_wf_ref : wf_constr_db.
+#[global] Hint Unfold MaybeInt_wf : wf_constr_db.
+#[global] Hint Resolve MaybeInt_eq : ref_constr_db.
 #[global] Hint Unfold Just : ref_constr_db.
 #[global] Hint Unfold Nothing : ref_constr_db.
-#[global] Hint Unfold Nothing : ref_constr_db.
-Definition mappend (lq_tmp0: Maybe) (lq_tmp1: Maybe): Maybe. 
+Definition mappend (lq_tmp0: MaybeInt) (lq_tmp1: MaybeInt): MaybeInt. 
 Proof. 
 	destruct lq_tmp0 as [lq_tmp0 lq_tmp0_p]. 
 	destruct lq_tmp1 as [lq_tmp1 lq_tmp1_p]. 
@@ -67,7 +59,7 @@ Proof.
 		refine (exist _ lq_tmp1 _); 
 		solver.  
 Defined. 
-Inductive mappend_rel : (Maybe_u -> (Maybe_u -> (Maybe_u -> Prop))) := 
+Inductive mappend_rel : (MaybeInt_u -> (MaybeInt_u -> (MaybeInt_u -> Prop))) := 
 	 | mappend_Nothing: (forall lq_tmp1 , mappend_rel Nothing_u lq_tmp1 lq_tmp1)
 	 | mappend_Just: (forall lq_tmp1 x , mappend_rel (Just_u x) lq_tmp1 (Just_u x)). 
 #[global] Hint Constructors mappend_rel : core_hint_db.
@@ -77,7 +69,7 @@ Inductive mappend_rel : (Maybe_u -> (Maybe_u -> (Maybe_u -> Prop))) :=
 #[global] Instance mappend_getF : getFunc mappend_rel := { 
 	getF' := mappend
 }.
-Definition mappend_rel_funct [lq_tmp0: Maybe_u] [lq_tmp1: Maybe_u]: (forall (VV: Maybe_u) (VV': Maybe_u) (H: mappend_rel lq_tmp0 lq_tmp1 VV) (K: mappend_rel lq_tmp0 lq_tmp1 VV') , VV = VV'). 
+Definition mappend_rel_funct [lq_tmp0: MaybeInt_u] [lq_tmp1: MaybeInt_u]: (forall (VV: MaybeInt_u) (VV': MaybeInt_u) (H: mappend_rel lq_tmp0 lq_tmp1 VV) (K: mappend_rel lq_tmp0 lq_tmp1 VV') , VV = VV'). 
 Proof. 
 	try revert lq_tmp1_p; generalize dependent lq_tmp1; 
 	induction lq_tmp0 as [(*Just*) x | (*Nothing*) ]; 
@@ -95,7 +87,7 @@ Proof.
 	rel_back' ( _nil). 
 Qed. 
 #[global] Hint Rewrite mappend_Just_lem : f_rel_back.
-Theorem mappend_rel_ex (lq_tmp0: Maybe_u) (lq_tmp1: Maybe_u) (lq_tmp0_p: (Maybe_wf lq_tmp0) /\ True) (lq_tmp1_p: (Maybe_wf lq_tmp1) /\ True): mappend_rel lq_tmp0 lq_tmp1 
+Theorem mappend_rel_ex (lq_tmp0: MaybeInt_u) (lq_tmp1: MaybeInt_u) (lq_tmp0_p: (MaybeInt_wf lq_tmp0) /\ True) (lq_tmp1_p: (MaybeInt_wf lq_tmp1) /\ True): mappend_rel lq_tmp0 lq_tmp1 
 		(⌊ mappend (exist _ lq_tmp0 lq_tmp0_p) (exist _ lq_tmp1 lq_tmp1_p) -⌋). 
 Proof. 
 	existence_lemma_pre mappend; 
@@ -110,7 +102,7 @@ Proof.
 Qed. 
 #[global] Hint Resolve mappend_rel_ex : rel_ax_db.
 Opaque mappend. 
-Theorem mappend__mappend_rel_rw (lq_tmp0: Maybe_u) (lq_tmp1: Maybe_u) (lq_tmp0_p: (Maybe_wf lq_tmp0) /\ True) (lq_tmp1_p: (Maybe_wf lq_tmp1) /\ True) (VV: Maybe_u): ((⌊ mappend (exist _ lq_tmp0 lq_tmp0_p) (exist _ lq_tmp1 lq_tmp1_p) -⌋) = VV) <-> (mappend_rel lq_tmp0 lq_tmp1 VV). 
+Theorem mappend__mappend_rel_rw (lq_tmp0: MaybeInt_u) (lq_tmp1: MaybeInt_u) (lq_tmp0_p: (MaybeInt_wf lq_tmp0) /\ True) (lq_tmp1_p: (MaybeInt_wf lq_tmp1) /\ True) (VV: MaybeInt_u): ((⌊ mappend (exist _ lq_tmp0 lq_tmp0_p) (exist _ lq_tmp1 lq_tmp1_p) -⌋) = VV) <-> (mappend_rel lq_tmp0 lq_tmp1 VV). 
 Proof. 
 	f__f_rel_rw. 
 Qed. 
@@ -119,18 +111,18 @@ Qed.
 #[global] Instance mappend_lookup_rw : dictionary rwLem mappend := { 
 	lookup' := mappend__mappend_rel_rw
 }.
-Theorem mappend__mappend_rel (lq_tmp0_r: Maybe) (lq_tmp1_r: Maybe) (VV: Maybe_u): ((⌊ mappend lq_tmp0_r lq_tmp1_r -⌋) = VV) <-> (mappend_rel (⌊ lq_tmp0_r -⌋) (⌊ lq_tmp1_r -⌋) VV). 
+Theorem mappend__mappend_rel (lq_tmp0_r: MaybeInt) (lq_tmp1_r: MaybeInt) (VV: MaybeInt_u): ((⌊ mappend lq_tmp0_r lq_tmp1_r -⌋) = VV) <-> (mappend_rel (⌊ lq_tmp0_r -⌋) (⌊ lq_tmp1_r -⌋) VV). 
 Proof. 
 	f__f_rel. 
 Qed. 
 #[global] Hint Rewrite mappend__mappend_rel : f_rel_funct_db.
-Theorem mappend__mappend_rel' (lq_tmp0: Maybe_u) (lq_tmp1: Maybe_u) (lq_tmp0_r: Maybe) (lq_tmp1_r: Maybe) (VV: Maybe_u): (lq_tmp0 = (⌊ lq_tmp0_r -⌋)) -> ((lq_tmp1 = (⌊ lq_tmp1_r -⌋)) -> (((⌊ mappend lq_tmp0_r lq_tmp1_r -⌋) = VV) <-> (mappend_rel lq_tmp0 lq_tmp1 VV))). 
+Theorem mappend__mappend_rel' (lq_tmp0: MaybeInt_u) (lq_tmp1: MaybeInt_u) (lq_tmp0_r: MaybeInt) (lq_tmp1_r: MaybeInt) (VV: MaybeInt_u): (lq_tmp0 = (⌊ lq_tmp0_r -⌋)) -> ((lq_tmp1 = (⌊ lq_tmp1_r -⌋)) -> (((⌊ mappend lq_tmp0_r lq_tmp1_r -⌋) = VV) <-> (mappend_rel lq_tmp0 lq_tmp1 VV))). 
 Proof. 
 	intros -> ->. 
 	refine (mappend__mappend_rel lq_tmp0_r lq_tmp1_r VV). 
 Qed. 
 #[global] Hint Resolve mappend__mappend_rel' : f_rel_funct_db.
-Definition mappend_rel_mk [lq_tmp0: Maybe_u] [lq_tmp1: Maybe_u] (lq_tmp0_p: (Maybe_wf lq_tmp0) /\ True) (lq_tmp1_p: (Maybe_wf lq_tmp1) /\ True): {VV: _ | mappend_rel lq_tmp0 lq_tmp1 VV}. 
+Definition mappend_rel_mk [lq_tmp0: MaybeInt_u] [lq_tmp1: MaybeInt_u] (lq_tmp0_p: (MaybeInt_wf lq_tmp0) /\ True) (lq_tmp1_p: (MaybeInt_wf lq_tmp1) /\ True): {VV: _ | mappend_rel lq_tmp0 lq_tmp1 VV}. 
 Proof. 
 	intros ; 
 	refine (subsumptionCast _ (fun (VV: _) => (mappend_rel lq_tmp0 lq_tmp1 VV)) 
@@ -139,11 +131,11 @@ Proof.
 	quicksolve. 
 Qed. 
 #[global] Hint Resolve mappend_rel_mk : f_rel_funct_db.
-#[global] Instance mappendPack : (@Pack (Maybe ::RT (fun (lq_tmp0_r: Maybe) => (Maybe ::RT (fun (lq_tmp1_r: Maybe) => nilRT)))) (Maybe_u ::UT (Maybe_u ::UT nilUT)) (ltac: (mkProjectsArgListTG (Maybe ::RT (fun (lq_tmp0_r: Maybe) => (Maybe ::RT (fun (lq_tmp1_r: Maybe) => nilRT)))) (Maybe_u ::UT (Maybe_u ::UT nilUT)))) Maybe_u (fun (x_38332132: (ArgList Maybe ::RT (fun (lq_tmp0_r: Maybe) => (Maybe ::RT (fun (lq_tmp1_r: Maybe) => nilRT))))) => (fun (v_x_38332132: Maybe_u) => (ltac: (flattenP (fun (lq_tmp0_r: Maybe) => (fun (lq_tmp1_r: Maybe) => (fun (VV: Maybe_u) => ((Maybe_wf VV) /\ True)))) x_38332132 v_x_38332132))))).
+#[global] Instance mappendPack : (@Pack (MaybeInt ::RT (fun (lq_tmp0_r: MaybeInt) => (MaybeInt ::RT (fun (lq_tmp1_r: MaybeInt) => nilRT)))) (MaybeInt_u ::UT (MaybeInt_u ::UT nilUT)) (ltac: (mkProjectsArgListTG (MaybeInt ::RT (fun (lq_tmp0_r: MaybeInt) => (MaybeInt ::RT (fun (lq_tmp1_r: MaybeInt) => nilRT)))) (MaybeInt_u ::UT (MaybeInt_u ::UT nilUT)))) MaybeInt_u (fun (x_60657082: (ArgList MaybeInt ::RT (fun (lq_tmp0_r: MaybeInt) => (MaybeInt ::RT (fun (lq_tmp1_r: MaybeInt) => nilRT))))) => (fun (v_x_60657082: MaybeInt_u) => (ltac: (flattenP (fun (lq_tmp0_r: MaybeInt) => (fun (lq_tmp1_r: MaybeInt) => (fun (VV: MaybeInt_u) => ((MaybeInt_wf VV) /\ True)))) x_60657082 v_x_60657082))))).
 Proof. 
 	buildPackG mappend mappend_rel mappend__mappend_rel mappend_rel_funct. 
 Defined.
-Definition mappend_assoc (xs: Maybe) (ys: Maybe) (zs: Maybe): {{forall (mappendres: Maybe_u), (mappend_rel (⌊ xs -⌋) (⌊ ys -⌋) mappendres) -> (forall (mappend_res_2: Maybe_u), (mappend_rel mappendres (⌊ zs -⌋) mappend_res_2) -> (forall (mappend_res_3: Maybe_u), (mappend_rel (⌊ ys -⌋) (⌊ zs -⌋) mappend_res_3) -> (forall (mappend_res_4: Maybe_u), (mappend_rel (⌊ xs -⌋) mappend_res_3 mappend_res_4) -> (mappend_res_2 == mappend_res_4))))}}. 
+Definition mappend_assoc (xs: MaybeInt) (ys: MaybeInt) (zs: MaybeInt): {{forall (mappendres: MaybeInt_u), (mappend_rel (⌊ xs -⌋) (⌊ ys -⌋) mappendres) -> (forall (mappend_res_2: MaybeInt_u), (mappend_rel mappendres (⌊ zs -⌋) mappend_res_2) -> (forall (mappend_res_3: MaybeInt_u), (mappend_rel (⌊ ys -⌋) (⌊ zs -⌋) mappend_res_3) -> (forall (mappend_res_4: MaybeInt_u), (mappend_rel (⌊ xs -⌋) mappend_res_3 mappend_res_4) -> (mappend_res_2 == mappend_res_4))))}}. 
 Proof. 
 	destruct xs as [xs xs_p]. 
 	destruct ys as [ys ys_p]. 
@@ -162,12 +154,12 @@ Proof.
 			refine (exist _ unit _); 
 			solver.   
 Defined. 
-Definition mempty: Maybe. 
+Definition mempty: MaybeInt. 
 Proof. 
 	refine (subsumptionCast _ _ Nothing _); 
 	solver. 
 Defined. 
-Inductive mempty_rel : (Maybe_u -> Prop) := 
+Inductive mempty_rel : (MaybeInt_u -> Prop) := 
 	 | mempty_def: mempty_rel Nothing_u. 
 #[global] Hint Constructors mempty_rel : core_hint_db.
 #[global] Instance mempty_lookup_rel : dictionary rel mempty := { 
@@ -176,7 +168,7 @@ Inductive mempty_rel : (Maybe_u -> Prop) :=
 #[global] Instance mempty_getF : getFunc mempty_rel := { 
 	getF' := mempty
 }.
-Definition mempty_rel_funct: (forall (VV: Maybe_u) (VV': Maybe_u) (H: mempty_rel VV) (K: mempty_rel VV') , VV = VV'). 
+Definition mempty_rel_funct: (forall (VV: MaybeInt_u) (VV': MaybeInt_u) (H: mempty_rel VV) (K: mempty_rel VV') , VV = VV'). 
 Proof. 
 	rel_functionhood_body. 
 Qed. 
@@ -196,7 +188,7 @@ Proof.
 Qed. 
 #[global] Hint Resolve mempty_rel_ex : rel_ax_db.
 Opaque mempty. 
-Theorem mempty__mempty_rel_rw (VV: Maybe_u): ((⌊ mempty -⌋) = VV) <-> (mempty_rel VV). 
+Theorem mempty__mempty_rel_rw (VV: MaybeInt_u): ((⌊ mempty -⌋) = VV) <-> (mempty_rel VV). 
 Proof. 
 	f__f_rel_rw. 
 Qed. 
@@ -205,12 +197,12 @@ Qed.
 #[global] Instance mempty_lookup_rw : dictionary rwLem mempty := { 
 	lookup' := mempty__mempty_rel_rw
 }.
-Theorem mempty__mempty_rel (VV: Maybe_u): ((⌊ mempty -⌋) = VV) <-> (mempty_rel VV). 
+Theorem mempty__mempty_rel (VV: MaybeInt_u): ((⌊ mempty -⌋) = VV) <-> (mempty_rel VV). 
 Proof. 
 	f__f_rel. 
 Qed. 
 #[global] Hint Rewrite mempty__mempty_rel : f_rel_funct_db.
-Theorem mempty__mempty_rel' (VV: Maybe_u): ((⌊ mempty -⌋) = VV) <-> (mempty_rel VV). 
+Theorem mempty__mempty_rel' (VV: MaybeInt_u): ((⌊ mempty -⌋) = VV) <-> (mempty_rel VV). 
 Proof. 
 	intros . 
 	refine (mempty__mempty_rel VV). 
@@ -224,13 +216,13 @@ Proof.
 	quicksolve. 
 Qed. 
 #[global] Hint Resolve mempty_rel_mk : f_rel_funct_db.
-Definition mempty_left (x: Maybe): {{forall (mappendres: Maybe_u), (mappend_rel (⌊ mempty -⌋) (⌊ x -⌋) mappendres) -> (mappendres = (⌊ x -⌋))}}. 
+Definition mempty_left (x: MaybeInt): {{forall (mappendres: MaybeInt_u), (mappend_rel (⌊ mempty -⌋) (⌊ x -⌋) mappendres) -> (mappendres = (⌊ x -⌋))}}. 
 Proof. 
 	destruct x as [x x_p]. 
 	refine (exist _ unit _); 
 	solver. 
 Defined. 
-Definition mempty_right (x: Maybe): {{forall (mappendres: Maybe_u), (mappend_rel (⌊ x -⌋) (⌊ mempty -⌋) mappendres) -> (mappendres = (⌊ x -⌋))}}. 
+Definition mempty_right (x: MaybeInt): {{forall (mappendres: MaybeInt_u), (mappend_rel (⌊ x -⌋) (⌊ mempty -⌋) mappendres) -> (mappendres = (⌊ x -⌋))}}. 
 Proof. 
 	destruct x as [x x_p]. 
 	induction x as [(*Just*) x | (*Nothing*) ]. 
@@ -241,56 +233,3 @@ Proof.
 		refine (exist _ unit _); 
 		solver.  
 Defined. 
-Inductive Maybe_u : Set := 
-	 | Just_u: Z -> Maybe_u
-	 | Nothing_u: Maybe_u
-	 | Nothing_u: Maybe_u. 
-Fixpoint Maybe_eq (x: Maybe_u) (y: Maybe_u): bool := 
-	match (x, y) with (Just_u x, Just_u x') => (true && (x ==? x')) | (Nothing_u, Nothing_u) => true | (Nothing_u, Nothing_u) => true | (_, _) => false end. 
-Definition Maybe_eq_refl: (forall (x: Maybe_u) , is_true (Maybe_eq x x)). 
-Proof. 
-	eq_refl. 
-Qed. 
-#[global] Hint Resolve Maybe_eq_refl : eq_hint_db.
-Definition Maybe_eqb_eq: (forall (s: Maybe_u) (t: Maybe_u) , (is_true (Maybe_eq s t)) -> (s = t)). 
-Proof. 
-	eqb_eq_lem. 
-Qed. 
-#[global] Hint Resolve Maybe_eqb_eq : eq_hint_db.
-#[global] Instance leibnitz_eq_Maybe : LeibnitzEqB := { 
-	equalB' := Maybe_eq;
-	refl' := Maybe_eq_refl;
-	eqb_eq' := Maybe_eqb_eq
-}.
-Fixpoint Maybe_wf (x: Maybe_u): Prop := 
-	match x with (Just_u VV) => True | Nothing_u => True | Nothing_u => True end. 
-Theorem Maybe_wf_ref [p: Maybe_u -> Prop] (tm: {v: Maybe_u | (Maybe_wf v) /\ (p v)}): Maybe_wf (⌊ tm -⌋). 
-Proof. 
-	destruct tm as [tm tm_p]. 
-	solver. 
-Qed. 
-Global Notation Maybe := {x: Maybe_u | (Maybe_wf x) /\ True}. 
-Definition Just_lem (VV: {VV: Z | True}): (Maybe_wf (Just_u (⌊ VV -⌋))) /\ True. 
-Proof. 
-	repeat first [split; solver]. 
-Defined. 
-Definition Just (VV: {VV: Z | True}): Maybe := 
-	exist _ (Just_u (⌊ VV -⌋)) (Just_lem VV). 
-Definition Nothing_lem: (Maybe_wf Nothing_u) /\ True. 
-Proof. 
-	repeat first [split; solver]. 
-Defined. 
-Definition Nothing: Maybe := 
-	exist _ Nothing_u Nothing_lem. 
-Definition Nothing_lem: (Maybe_wf Nothing_u) /\ True. 
-Proof. 
-	repeat first [split; solver]. 
-Defined. 
-Definition Nothing: Maybe := 
-	exist _ Nothing_u Nothing_lem. 
-#[global] Hint Resolve Maybe_wf_ref : wf_constr_db.
-#[global] Hint Unfold Maybe_wf : wf_constr_db.
-#[global] Hint Resolve Maybe_eq : ref_constr_db.
-#[global] Hint Unfold Just : ref_constr_db.
-#[global] Hint Unfold Nothing : ref_constr_db.
-#[global] Hint Unfold Nothing : ref_constr_db.
